experiment without option

src/TMP/Task/Equivalence.v
@@ -82,9 +82,39 @@ Fixpoint mesure_val (v : Value) : nat :=
   | VMap l => 1 + (mesure_val_map l)
   end.
 
+
+
+Definition mesure_exp_env (e : Expression) (env : Environment) : nat :=
+  let
+    sum_nat (l : list nat) : nat :=
+      fold_left Nat.add l 0
+  in
+  let 
+    mesure_val_env (env : Environment) : nat :=
+      sum_nat (map (fun '(x, y) => (mesure_val y)) env)
+  in
+  (mesure_exp e) + (mesure_val_env env).
+
+
+Definition mesure_val_list (vl : list Value) : nat :=
+  let
+    sum_nat (l : list nat) : nat :=
+      fold_left Nat.add l 0
+  in
+  sum_nat (map mesure_val vl).
+
+Definition mesure_exp_list (el : list Expression) : nat :=
+  let
+    sum_nat (l : list nat) : nat :=
+      fold_left Nat.add l 0
+  in
+  sum_nat (map mesure_exp el).
+
 (*{measure (mesure_val v)} *)
 
+(*
 Program Fixpoint val_to_exp (v : Value) {measure (mesure_val v)} : option Expression :=
+  (*
   let
     val_to_exp_map (x y : Value) : option (Expression * Expression) :=
       match (val_to_exp x), (val_to_exp y) with
@@ -92,31 +122,35 @@ Program Fixpoint val_to_exp (v : Value) {measure (mesure_val v)} : option Expres
       | _, _ => None
       end
   in
+  *)
   match v with
   | VNil => Some ENil
   | VLit l => Some (ELit l)
   (*TODO*)
-  | VClos env ext id vl e fid => None(*match (subst_env (EFun vl e) env) with
+  | VClos env ext id vl e fid => None (*match (subst_env (EFun vl e) env) with
                               | Some e' => Some (EFun vl e')
                               | None => None
-                              end *)
+                              end*)
   | VCons hd tl => match (val_to_exp hd), (val_to_exp tl) with
                   | Some hd', Some tl' => Some (ECons hd' tl')
                   | _, _ => None
                   end
-  | VTuple l => match (mapM val_to_exp l) with
-                | Some l' => Some (ETuple  l')
+  | VTuple l => match (@mapM option _ _ (fun (x : Value) => val_to_exp x : option Expression) l : option (list Expression)) with
+                | Some l' => Some (ETuple l')
                 | None => None
                 end
-  | VMap l =>  match (mapM (fun '(x, y) => val_to_exp_map x y) l) with
+  | VMap l =>  match (@mapM option _ _ (fun '(x, y) => match (val_to_exp x), (val_to_exp y) with
+                                          | Some x', Some y' => Some (x', y')
+                                          | _, _ => None
+                                          end) l : option (list (Expression * Expression))) with
               | Some l' => Some (EMap l')
               | None => None
               end
-  end
+  end.
 
-with 
+(*with *)
 
-subst_env (e : Expression) (Γ : Environment) : option Expression :=
+Fixpoint subst_env (e : Expression) (Γ : Environment) : option Expression :=
   let
     subst_env_case (pl : list Pattern) (g : Expression) (b : Expression) : option (list Pattern * Expression * Expression) :=
       match (subst_env g Γ), (subst_env b Γ) with
@@ -202,7 +236,180 @@ subst_env (e : Expression) (Γ : Environment) : option Expression :=
                               | _, _, _ => None
                               end
   end.
+*)
+
+(*
+ELetRec (l : list (FunctionIdentifier * ((list Var) * Expression))) 
+        (e : Expression)
+(ext : list (nat * FunctionIdentifier * FunctionExpression))
+FunctionExpression: 
+*)
+
+(*
+Program Fixpoint val_to_exp2 (v : Value) {measure (mesure_val v)} : Expression :=
+  match v with
+  | VNil => ENil
+  | VLit l => ELit l
+  | VClos env ext id vl e fid => EFun vl e
+  | VCons hd tl => ECons (val_to_exp2 hd) (val_to_exp2 tl)
+  | VTuple l => ETuple (map (fun x => val_to_exp2 x) l)
+  | VMap l =>  EMap (map (fun '(x, y) => (val_to_exp2 x, val_to_exp2 y)) l)
+  end.
+  Next Obligation.
+    intros. rewrite <- Heq_v. simpl. lia.
+  Qed.
+  Next Obligation.
+    intros. rewrite <- Heq_v. simpl. lia.
+  Qed.
+  Next Obligation.
+    intro. induction l. intros. admit. (*mesure_val x < mesure_val v*)
+  Admitted.
+  Next Obligation.
+    intro. induction l. admit.
+  Admitted.
+  Next Obligation.
+    intro. induction l. admit.
+  Admitted.
+  Next Obligation.
+    admit.
+  Admitted.
+*)
+
+Program Fixpoint val_to_exp2 (v : Value) {measure (mesure_val v)} : Expression :=
+  let
+    fix list_to_exp (vl : list Value) (el : list Expression) : list Expression :=
+      match vl with 
+      | [] => el
+      | hd :: tl => list_to_exp tl (el ++ [val_to_exp2 hd])
+      end
+  in
+  let
+    fix map_to_exp (vl : list (Value * Value)) (el : list (Expression * Expression)) : list (Expression * Expression) :=
+      match vl with 
+      | [] => el
+      | hd :: tl => map_to_exp tl (el ++ [(val_to_exp2 (fst hd), val_to_exp2 (snd hd))])
+      end
+  in
+  match v with
+  | VNil => ENil
+  | VLit l => ELit l
+  | VClos env ext id vl e fid => EFun vl e
+  | VCons hd tl => ECons (val_to_exp2 hd) (val_to_exp2 tl)
+  | VTuple l => ETuple (list_to_exp l [])
+  | VMap l =>  EMap (map_to_exp l [])
+  end.
+  Next Obligation.
+    intros. admit.
+  Admitted.
+  Next Obligation.
+    intros. admit.
+  Admitted.
+  Next Obligation.
+    intros. admit.
+  Admitted.
+  Next Obligation.
+    intros. rewrite <- Heq_v. simpl. lia.
+  Admitted.
+  Next Obligation.
+    intros. rewrite <- Heq_v. simpl. lia.
+  Admitted.
+  Next Obligation.
+    intros. simpl. unfold well_founded. intros. constructor. intros. constructor. intros. admit.
+  Admitted.
+
+
+Fixpoint subst_env2 (e : Expression) (Γ : Environment) : Expression :=
+  match e with
+  | EValues el => map (fun x => subst_env2 x Γ) el
+  | ENil => ENil
+  | ELit l => ELit l
+  | EVar v => match (get_value Γ (inl v)) with
+              | Some [v'] => val_to_exp2 v'
+              | _ => EVar v
+              end
+  | EFunId f =>  match (get_value Γ (inr f)) with
+                | Some [f'] => val_to_exp2 f'
+                | _ => EFunId f
+                end
+  | EFun vl e => EFun vl (subst_env2 e Γ)
+  | ECons hd tl => ECons (subst_env2 hd Γ) (subst_env2 tl Γ)
+  | ETuple l => ETuple (map (fun x => subst_env2 x Γ) l)
+  | ECall m f l => ECall (subst_env2 m Γ) (subst_env2 f Γ) (map (fun x => subst_env2 x Γ) l)
+  | EPrimOp f l => EPrimOp f (map (fun x => subst_env2 x Γ) l)
+  | EApp exp l => EApp (subst_env2 exp Γ) (map (fun x => subst_env2 x Γ) l)
+  | ECase e l => ECase (subst_env2 e Γ) (map (fun '(pl, g, b) => pl, (subst_env2 g Γ), (subst_env2 b Γ)) l)
+  | ELet l e1 e2 => ELet l (subst_env2 e1 Γ) (subst_env2 e2 Γ)
+  | ESeq e1 e2 => ESeq (subst_env2 e1 Γ) (subst_env2 e2 Γ)
+  | ELetRec l e => ELetRec (map (fun '(fid, (vl, b)) => fid, (vl, (subst_env2 b Γ))) l) (subst_env2 e Γ)
+  | EMap l => EMap (map (fun '(x, y) => (subst_env2 x Γ), (subst_env2 y Γ)) l)
+  | ETry e1 vl1 e2 vl2 e0 => ETry (subst_env2 e1 Γ) vl1 (subst_env2 e2 Γ) vl2 (subst_env2 e0 Γ)
+  end.
 
 
 
+Definition mesure1 (v : Value) (vltuple : (list Value)) (eltuple : (list Expression)) : nat :=
+  (mesure_val v) + (mesure_val_list vltuple) + (mesure_exp_list eltuple).
+
+Program Fixpoint val_to_exp3 (v : Value) (vltuple : (list Value)) (eltuple : (list Expression)) {measure (mesure1 v vltuple eltuple)} : Expression :=
+  match eltuple with
+  | [] => match v with
+          | VNil => ENil
+          | VLit l => ELit l
+          | VClos env ext id vl e fid => EFun vl e
+          | VCons hd tl => ECons (val_to_exp3 hd [] []) (val_to_exp3 tl [] [])
+          | VTuple l => ETuple []
+          | VMap l =>  EMap []
+          end
+  | hd :: tl => match vltuple with
+                | [] => ETuple (eltuple ++ [val_to_exp3 v [] []])
+                | hd' :: tl' => val_to_exp3 hd' tl' (eltuple ++ [val_to_exp3 v [] []])
+                end
+  end.
+  Next Obligation.
+    intros. simpl. rewrite <- Heq_v. rewrite <- Heq_eltuple. simpl. admit.
+  Admitted.
+  Next Obligation.
+    intros. simpl. rewrite <- Heq_v. rewrite <- Heq_eltuple. simpl. admit.
+  Admitted.
+  Next Obligation.
+    intros. simpl. rewrite <- Heq_vltuple. rewrite <- Heq_eltuple. simpl.  admit.
+  Admitted.
+  Next Obligation.
+    intros. simpl. rewrite <- Heq_vltuple. rewrite <- Heq_eltuple. simpl. admit.
+  Admitted.
+  Next Obligation.
+    intros. simpl. admit.
+  Admitted.
+  Next Obligation.
+    intros. simpl. admit.
+  Admitted.
+  (*
+  match v with
+  | VNil => ENil
+  | VLit l => ELit l
+  | VClos env ext id vl e fid => EFun vl e
+  | VCons hd tl => ECons (val_to_exp3 hd [] []) (val_to_exp3 tl [] [])
+  | VTuple l => match l with
+                | [] => ETuple eltuple
+                | hd :: tl => ENil
+                end
+  | VMap l =>  EMap []
+  end.
+  *)
+  (*
+  match vltuple with
+  | [] => match v with
+          | VNil => ENil
+          | VLit l => ELit l
+          | VClos env ext id vl e fid => EFun vl e
+          | VCons hd tl => ECons (val_to_exp3 hd [] []) (val_to_exp3 tl [] [])
+          | VTuple l => ETuple []
+          | VMap l =>  EMap []
+          end
+  | hd :: tl => match v with
+                | VTuple l => ENil
+                | _ => ENil
+                end
+  end.
+  *)
 End SubstEnviroment.
